ConNF/FOA/Basic.lean
@@ -1,5 +1,5 @@
 import ConNF.FOA.Basic.CompleteOrbit
 import ConNF.FOA.Basic.Sublitter
 import ConNF.FOA.Basic.Hypotheses
-import ConNF.FOA.Basic.Constrains
 import ConNF.FOA.Basic.Flexible
+import ConNF.FOA.Basic.Constrains
