ConNF/FOA/Basic/Flexible.lean
@@ -1,4 +1,4 @@
-import ConNF.FOA.Basic.Constrains
+import ConNF.FOA.Basic.Hypotheses
 
 open Quiver Set Sum WithBot
 
@@ -27,24 +27,6 @@ def Flexible (A : ExtendedIndex β) (L : Litter) : Prop :=
 
 theorem flexible_cases (A : ExtendedIndex β) (L : Litter) : Inflexible A L ∨ Flexible A L :=
   or_not
-
-theorem not_constrains_flexible {β : Λ} (c : Address β)
-    {A : ExtendedIndex β} {L : Litter} (hL : Flexible A L) :
-    ¬c ≺ ⟨A, inr L.toNearLitter⟩ := by
-  rintro (⟨A, a⟩ | ⟨A, N, hN⟩ | ⟨A, N, a, ha⟩ | ⟨hδ, hε, hδε, A, t, c, hc⟩ | ⟨hε, A, a⟩)
-  · exact hN (NearLitter.IsLitter.mk _)
-  · obtain (ha | ha) := ha
-    · cases ha.2 ha.1
-    · cases ha.2 ha.1
-  · exact hL (Inflexible.mk_coe hδ hε hδε _ _)
-  · exact hL (Inflexible.mk_bot hε _ _)
-
-theorem not_transConstrains_flexible {β : Λ} (c : Address β)
-    {A : ExtendedIndex β} {L : Litter} (hL : Flexible A L) :
-    ¬c < ⟨A, inr L.toNearLitter⟩ := by
-  intro h
-  obtain ⟨d, _, hd⟩ := Relation.TransGen.tail'_iff.mp h
-  exact not_constrains_flexible d hL hd
 
 theorem mk_flexible (A : ExtendedIndex β) : #{L | Flexible A L} = #μ := by
   refine le_antisymm ((Cardinal.mk_subtype_le _).trans mk_litter.le) ?_
@@ -228,13 +210,6 @@ theorem InflexibleBotPath.comp_B (h : InflexibleBotPath B) (A : Path (β : TypeI
   rfl
 
 end Comp
-
-theorem InflexibleBot.constrains {β : Λ} {A : ExtendedIndex β} {L : Litter}
-    (h : InflexibleBot A L) :
-    (⟨h.path.B.cons (bot_lt_coe _), inl h.a⟩ : Address β) < ⟨A, inr L.toNearLitter⟩ := by
-  have := Constrains.fuzzBot h.path.hε h.path.B h.a
-  rw [← h.hL, ← h.path.hA] at this
-  exact Relation.TransGen.single this
 
 @[aesop unsafe 50% apply]
 theorem inflexible_of_inflexibleBot {β : Λ} {A : ExtendedIndex β} {L : Litter}
